theories/Syntax.v
@@ -1,4 +1,5 @@
 From Coq Require Import Unicode.Utf8_core.
+From Coq Require Import Peano Nat Arith Lia.
 From TLC Require Import LibLN LibTactics LibFset.
 From TTSB Require Import Tactics.
 
@@ -11,16 +12,16 @@ Inductive term :=
   | TmApp : term -> term -> term 
 .
 
-Reserved Notation "{ k ~> u } t" (at level 67).
+Reserved Notation "[{ k ~> u }] t" (at level 67).
 Fixpoint open' (k : nat) (u : term) (t : term) : term :=
   match t with 
   | TmBVar i => If i = k then u else t 
   | TmFVar y => t
-  | TmAbs t' => TmAbs ({ (S k) ~> u } t')
-  | TmApp t1 t2 => TmApp ({k ~> u} t1) (({k ~> u} t2))
+  | TmAbs t' => TmAbs ([{ (S k) ~> u }] t')
+  | TmApp t1 t2 => TmApp ([{k ~> u}] t1) (([{k ~> u}] t2))
   end
   where 
-  "{ k ~> u } t" := (open' k u t)
+  "[{ k ~> u }] t" := (open' k u t)
   .
 Definition open : term -> term -> term := open' 0.
 Notation " t ^^ u " := (open u t) (at level 67).
@@ -39,14 +40,16 @@ Inductive lc : term -> Prop :=
       ∀ (x : var), 
       lc (TmFVar x) 
   | LCAbs : 
-      ∀ (t : term), 
-      (∀ (x : var), (x \notin fv t) -> lc (t ^ x)) -> 
+      ∀ (L : vars) (t : term), 
+      (∀ (x : var), (x \notin L) -> lc (t ^ x)) -> 
       lc (TmAbs t)
   | LCApp : 
       ∀ (t1 t2 : term),
       lc t1 -> lc t2 ->
       lc (TmApp t1 t2)
 .
+#[global]
+Hint Constructors lc : core.
 
 
 
@@ -86,4 +89,217 @@ Proof.
   generalize 0.
   intros n t; gen n.
   induction* t; introv Hnotin; repeat (simpls || reduce_max || case_if); fequals*.
+Qed.
+
+
+Section term_size_ind.
+  Inductive le_type : nat -> nat -> Type :=
+  | O_le_n : ∀ n, le_type 0 n
+  | Sn_le_Sm : ∀ n m, le_type n m -> le_type (S n) (S m)
+  .
+
+  Lemma le_refl :
+    ∀ a, le_type a a.
+  Proof.
+    hint O_le_n, Sn_le_Sm.
+    intro.
+    induction* a.
+  Qed.
+
+  Lemma le_trans : 
+    ∀ a b c, le_type a b -> le_type b c -> le_type a c.
+  Proof with autos*.
+    hint O_le_n, Sn_le_Sm.
+    intro a.
+    inductions a;
+    introv Hlt_a_b Hlt_b_c;
+    inverts Hlt_a_b;
+    inverts* Hlt_b_c.
+  Qed.
+
+  Lemma le_S : 
+    ∀ a, le_type a (S a).
+  Proof.
+    hint O_le_n, Sn_le_Sm.
+    intro.
+    induction* a.
+  Qed.
+  (* Inductive or_type A B : Type :=
+  | ort_intro_l : A -> or_type A B
+  | ort_intro_r : B -> or_type A B
+  . *)
+
+  Definition lt_type n m := le_type (S n) m.
+
+  Variable P : term -> Type.
+
+  Definition max (a b : nat) :=
+    if leb a b then b else a.
+
+  Lemma max_comm : 
+    ∀ a b, max a b = max b a.
+  Proof.
+    intros.
+    induction a; unfold max; destruct b; simpls*.
+    destruct (a <=? b) eqn:Heqaleb; destruct (b <=? a) eqn:Hblea;
+    autos.
+    - apply leb_complete in Heqaleb, Hblea. lia.
+    - apply leb_complete_conv in Heqaleb, Hblea. lia.
+  Qed.
+
+  Lemma le_max_self :
+    ∀ a b, le_type a (max a b).
+  Proof.
+    hint le_refl, O_le_n, Sn_le_Sm.
+    induction a; intros; unfolds max; destruct b; simpls*; case_if; substs*.
+    specialize IHa with b. rewrite* C in IHa.
+  Qed.
+
+  Fixpoint size_for_ind (t : term) :=
+    match t with 
+    | TmBVar _ => 0
+    | TmFVar _ => 0
+    | TmAbs t => S (size_for_ind t)
+    | TmApp t1 t2 => 1 + max (size_for_ind t1) (size_for_ind t2)
+    end.
+
+  Lemma size_for_ind_open : 
+    ∀ t x, 
+    size_for_ind t = size_for_ind (t ^ x).
+  Proof.
+    unfold "^"; generalize 0.
+    intros n t; gen n.
+    induction* t; intros; repeat (case_if || simpls || substs); autos.
+  Qed.
+
+  Hypothesis H : forall t, (forall t', lt_type (size_for_ind t') (size_for_ind t) -> P t') -> P t.
+
+
+  Theorem term_size_ind : forall xs, P xs.
+  Proof.
+    asserts H_ind : (
+      ∀ t t', 
+          (le_type (size_for_ind t') (size_for_ind t)) -> P t'
+    ).
+    
+      
+    {
+      hint le_trans.
+      intro t; inductions t; intros t' Hlen; apply H; intros l0 H0; simpls;
+      inverts Hlen;
+      match goal with 
+      | [ H : _ = size_for_ind _ |- _] => 
+          rewrite <- H in *; clear H
+      end; inverts* H0.
+      unfolds max; simpls*. case_if.
+      - apply IHt2.
+        apply le_trans with n.
+        + assumption.
+        + assumption.
+      - apply IHt1.
+        apply le_trans with n.
+        + assumption.
+        + assumption.
+    }
+    intros t.
+    apply H_ind with (t := t).
+    apply le_refl.
+  Qed.
+
+
+End term_size_ind.
+
+#[global]
+Hint Extern 1 (lt_type (size_for_ind (_ ^ _))  _) => 
+  rewrite <- size_for_ind_open; apply le_refl : core.
+#[global]
+Hint Extern 1 (lt_type _  (S (max _ _))) => 
+  apply Sn_le_Sm; try solve[apply le_max_self]; rewrite max_comm; apply le_max_self : core.
+
+Local Ltac gather_vars := 
+  let A := gather_vars_with (fun x : vars => x) in 
+  let B := gather_vars_with (fun x : var => \{x}) in 
+  let C := gather_vars_with (fun x : term => fv x) in 
+  constr:(A \u B \u C).
+
+Local Ltac pick_fresh x :=
+  let L := gather_vars in pick_fresh_gen L x.
+
+Fixpoint is_free_BVar (n : nat) (t : term) :=
+  match t with
+  | TmBVar k => n = k
+  | TmFVar _ => False 
+  | TmAbs t' => is_free_BVar (S n) t'
+  | TmApp t1 t2 => is_free_BVar n t1 \/ is_free_BVar n t2 
+  end.
+
+Lemma free_bvar_neq : 
+  ∀ t n k x, 
+  k ≠ n ->
+  is_free_BVar (n) t -> 
+  is_free_BVar (n) ([{k ~> TmFVar x}] t).
+Proof.
+  intros t.
+  induction t; introv Hneq Hfree; repeat (simpls || case_if); autos*.
+Qed.
+Lemma lc_no_free_bvar :
+  ∀ t,
+  lc t -> 
+  ∀ n, ¬ is_free_BVar n t.
+Proof.
+  intro t.
+  induction t using term_size_ind; destruct t; intros Hlc k Hfree; simpls*.
+  - inversion Hlc.
+  - inverts Hlc.
+    pick_fresh x.
+    apply H with (t' := t ^ x) (n := S k).
+    + rewrite <- size_for_ind_open; simpls; constructor; apply le_refl.
+    + apply* H1.
+    + unfold "^". apply* free_bvar_neq.
+  - reduce_max; inverts Hlc.
+    + eapply H with (t' := t1) (n:=k); try assumption.
+      constructor. apply le_max_self.
+    + eapply H with (t' := t2) (n:=k); try assumption.
+      constructor. rewrite max_comm. apply le_max_self.
+Qed.
+
+Lemma free_Bvar_open :
+  ∀ t p n, 
+  ¬ is_free_BVar n t ->
+  [{n ~> p}] t = t.
+Proof.
+  induction t; introv Hnfree; repeat (simpls || case_if); autos*.
+  - fequals*.
+  - fequals*.
+Qed.
+
+
+Lemma lc_open_substs : 
+  ∀ t p x y, lc p -> x ≠ y -> ([y ~> p]t) ^ x = [y ~> p](t ^ x).
+Proof.
+  unfold "^"; generalize 0.
+  introv Hlc Hneq. gen n.
+  inductions t; intros; repeat (case_if || reduce_max || simpls || substs); autos*.
+  - apply free_Bvar_open.
+    apply* lc_no_free_bvar.
+  - fequals.
+    apply* IHt.
+  - fequals. 
+    + rewrite* IHt1.
+    + rewrite* IHt2.
+Qed.
+
+
+Lemma lc_open_diff : 
+  ∀ t p x k, k ≠ 0 -> lc p -> ([{k ~> p}] t) ^ x = [{k ~> p}](t ^ x).
+Proof.
+  unfold "^". generalize 0.
+  introv Hneq Hlc; gen n k x p.
+  inductions t; intros; repeat (case_if || reduce_max || simpls || substs); autos*.
+  - apply free_Bvar_open, lc_no_free_bvar. assumption.
+  - fequals.
+    apply* IHt.
+  - fequals. 
+    + rewrite* IHt1.
+    + rewrite* IHt2.
 Qed.
